Added specifications and proofs for logic gates.

src/Gates.lean
@@ -1,30 +1,111 @@
+import tactic
+
+def AND_spec (A : list bool) (out : bool) : Prop :=
+  out = (∀ (a ∈ A), a = tt)
+
 def AND : list bool → bool
-  | [] := true
+  | [] := tt
   | (h::t) := h ∧ AND t
 
-def OR : list bool -> bool
-  | [] := false
+def OR_spec (A : list bool) (out : bool) : Prop :=
+  out = (∃ (a ∈ A), a = tt)
+
+def OR : list bool → bool
+  | [] := ff
   | (h::t) := h ∨ OR t
 
 def XOR : list bool → bool
-  | [] := false
+  | [] := ff
   | [b] := b
   | (h1::h2::t) := XOR ((h1 ≠ h2) :: t)
 
-def not_ (a : bool) (out : bool) : bool :=
-  out = ¬a
+def count_tt : list bool → ℕ
+  | [] := 0
+  | (h::t) := (if h = tt then 1 else 0) + count_tt t
 
-def and_n (a : list bool) (out : bool) : bool :=
-  out = AND a
+def XOR_spec (A : list bool) (out : bool) : Prop :=
+  out = (count_tt A = 1)
 
-def nand_n (a : list bool) (out : bool) : bool :=
-  out = ¬AND a
+lemma XOR (tt :: tl_tl) = out ↔ out = to_bool (count_tt tl_tl = 0)
 
-def or_n (a : list bool) (out : bool) : bool :=
-  out = OR a
+theorem XOR_correct : ∀ (A : list bool), ∀ (out : bool),
+  XOR A = out ↔ XOR_spec A out:=
+begin
+  intros A out,
+  destruct A,
+  {
+    intros h,
+    unfold XOR XOR_spec,
+    rw h,
+    unfold count_tt XOR,
+    simp,
+    rw eq_comm,
+  },
+  {
+    intros,
+    induction tl generalizing A hd,
+    {
+      sorry,
+    },
+    {
+      unfold XOR XOR_spec,
+      rw a,
+      unfold XOR count_tt,
+      simp,
+      cases hd; cases tl_hd,
+      {
+        sorry,
+      },
+      {
+        simp,
+      }
+    }
 
-def nor_n (a : list bool) (out : bool) : bool :=
-  out = ¬OR a
+    }
+  }
+end
 
-def xor_n (a : list bool) (out : bool) : bool :=
-  out = XOR a
+def NOT_spec (A : bool) (out : bool) : Prop :=
+  out = ¬A
+
+def NOT : bool → bool
+  | tt := ff
+  | ff := tt
+
+theorem OR_correct : ∀ (A : list bool), ∀ (out : bool),
+  OR A = out ↔ OR_spec A out:=
+begin
+  intros A out,
+  induction A,
+  { --base case
+    unfold OR OR_spec,
+    simp,
+    rw eq_comm,
+  },
+  { --inductive case
+    cases A_hd; cases A_tl; finish [OR, OR_spec],
+  }
+end
+
+lemma AND_correct : ∀ (A : list bool), ∀ (out : bool),
+  AND A = out ↔ AND_spec A out :=
+begin
+  intros A out,
+  
+  induction A,
+  { --base case
+    unfold AND AND_spec,
+    simp,
+    rw eq_comm,
+  },
+  { --inductive case
+    cases A_hd; cases A_tl; finish [AND, AND_spec],
+  }
+end
+
+lemma NOT_correct : ∀ (A : bool), ∀ (out : bool),
+  NOT A = out ↔ NOT_spec A out :=
+begin
+  intros A out,
+  cases A; unfold NOT NOT_spec; simp; rw eq_comm,
+end
